src/theories/PolyFirstOrder.v
@@ -12,13 +12,13 @@ Section PolySyntax.
 Definition ty_ctx := nat.
 Context (sig_sorts : nat -> Type).
 
-Inductive ty_valu : ty_ctx -> snoc_list Type -> Type := 
+Inductive ty_valu {T: Type} : ty_ctx -> snoc_list T -> Type := 
 | TVEmp : 
-  ty_valu 0 (SLNil _)
+  ty_valu 0 SLNil
 | TVSnoc : 
-  forall ctx T sl, 
+  forall ctx t sl, 
     ty_valu ctx sl -> 
-    ty_valu (S ctx) (Snoc _ sl T).
+    ty_valu (S ctx) (Snoc sl t).
 
 Inductive ty_ctx_var: ty_ctx -> Type :=
 | TCVHere:
@@ -59,65 +59,27 @@ Definition ctx t_ctx := snoc_list (ty_expr t_ctx 0).
 Inductive var: forall t_ctx, ctx t_ctx -> ty_expr t_ctx 0 -> Type := 
 | VHere:
   forall t_ctx (c: ctx t_ctx) e,
-    var t_ctx (Snoc _ c e) e
+    var t_ctx (Snoc c e) e
 | VThere:
   forall t_ctx (c: ctx t_ctx) s s',
     var t_ctx c s' ->
-    var _ (Snoc _ c s) s'.
+    var _ (Snoc c s) s'.
 Derive Signature NoConfusion for var.
-
-(* Definition infer_args_ty t_parent t_child c_parent c_child args args' (parent_args : HList.t (tm t_parent c_parent) args) : HList.t (tm t_child c_child) args'. Admitted. *)
-
-(* Definition lift_return t_parent t_child c_parent c_child *)
 
 Context (sig: signature).
 
-(* TODO:
-    add type variables here, 
-    calculate return type from type variables and function signature,
-    calculate type of argument variables from type variables and function signature
 
-  e.g.
-
-    (forall A B (a: A) (b: B), A * B) [X, Y] => 
-    args = X, Y
-    ret = X * Y
+(* A list of type expressions in an outer context, with same size as an inner context.
+   The type indices are:
+    type_params t_outer t_inner t_exprs
 *)
 
-Inductive ty_params t_ctx_outer : ty_ctx -> snoc_list (ty_expr t_ctx_outer 0) -> Type := 
-| TPEmp : 
-  ty_params t_ctx_outer 0 (SLNil _)
-| TPSnoc : 
-  forall ctx te sl, 
-    ty_params t_ctx_outer ctx sl -> 
-    ty_params t_ctx_outer (S ctx) (Snoc _ sl te).
-
-(* Definition infer_ 
-
-  ty_expr t_ctx_inner 0 -> 
-  ty_args -> 
-
-  ty_expr t_ctx_outer 0
-*)
-
-(* 
-
-  append has function type 
-    forall A,
-      A -> A -> A
-
-  
-
-*)
-
-(* True but not needed *)
-Definition insert_closed t_ctx n (te: ty_expr 0 n) : ty_expr t_ctx n.
-Admitted.
+Definition ty_params t_ctx_outer := @ty_valu (ty_expr t_ctx_outer 0).
 
 Equations lookup_tp_var t_ctx_outer t_ctx_inner tys (tp: ty_params t_ctx_outer t_ctx_inner tys) (tc_var: ty_ctx_var t_ctx_inner) : ty_expr t_ctx_outer 0 := {
-  lookup_tp_var _ _ _ (TPSnoc _ e _ _) (TCVHere _) := 
+  lookup_tp_var _ _ _ (TVSnoc _ e _ _) (TCVHere _) := 
     e; 
-  lookup_tp_var _ _ _ (TPSnoc _ _ _ tv') (TCVThere _ tc_var') := 
+  lookup_tp_var _ _ _ (TVSnoc _ _ _ tv') (TCVThere _ tc_var') := 
     lookup_tp_var _ _ _ tv' tc_var'; 
 }.
 
@@ -143,38 +105,8 @@ Inductive tm t_ctx : ctx t_ctx -> ty_expr t_ctx 0 -> Type :=
   forall t_ctx' t_args c args ret,
     sig.(sig_funs) t_ctx' args ret ->
     forall (ty_args : ty_params t_ctx t_ctx' t_args), (* type arguments *)
-      HList.t (fun te => tm t_ctx c (apply_ty_args _ _ _ _ ty_args te)) args -> 
-      tm t_ctx c (apply_ty_args _ _ _ _ ty_args ret). 
-
-
-    (* 
-      append : forall A (a: list A) (a': list A), A
-
-      @append B : forall (a: list B) (a': list B), B
-
-      B (bs: list B)
-
-      append bs bs = ...
-
-      @append B bs bs
-    
-    *)
-    (* append: demo_funs 1 [list_A; list_A] list_A 
-
-      this is what we have defined right now: 
-
-      append -> 
-      [list_A; list_A] -> 
-      tm ...
-
-      in a polymorphic setting, what we actually want is:
-
-      (fun A => append ) -> 
-      X -> 
-      [list_X; list_X] -> 
-      tm ... a term in which X and list_X are defined
-    *)
-
+      HList.t (tm t_ctx c) (List.map (apply_ty_args t_ctx' t_ctx t_args 0 ty_args) args) -> 
+      tm t_ctx c (apply_ty_args t_ctx' t_ctx t_args 0 ty_args ret). 
 
 Derive Signature for tm.
 
@@ -190,10 +122,11 @@ Inductive fm t_ctx : ctx t_ctx -> Type :=
     fm t_ctx c
 (* A relation (with arguments) *)
 | FRel:
-  forall c args,
-    sig.(sig_rels) t_ctx args ->
-    HList.t (tm t_ctx c) args ->
-    fm t_ctx c 
+  forall t_ctx' t_args c args,
+    sig.(sig_rels) t_ctx' args ->
+    forall (ty_args : ty_params t_ctx t_ctx' t_args), (* type arguments *)
+      HList.t (tm t_ctx c) (List.map (apply_ty_args t_ctx' t_ctx t_args 0 ty_args) args) -> 
+      fm t_ctx c 
 (* Negation, disjunction, conjunction, and implication *)
 | FNeg: forall c, fm t_ctx c -> fm t_ctx c
 | FOr: forall c, fm t_ctx c -> fm t_ctx c -> fm t_ctx c
@@ -203,18 +136,18 @@ Inductive fm t_ctx : ctx t_ctx -> Type :=
 (* Quantification *)
 | FForall:
   forall c s,
-    fm t_ctx (Snoc _ c s) ->
+    fm t_ctx (Snoc c s) ->
     fm t_ctx c
 | FExists:
   forall c s,
-    fm t_ctx (Snoc _ c s) ->
+    fm t_ctx (Snoc c s) ->
     fm t_ctx c.
 Derive Signature for fm.
 
 Inductive poly_fm : ty_ctx -> Type := 
 | PFm : 
   forall tc, 
-    fm tc (SLNil _ ) -> 
+    fm tc SLNil -> 
     poly_fm tc
 | PForall : 
   forall tc, 
@@ -236,29 +169,80 @@ Context `(interp_sorts : forall n, sig_sorts n -> arity_ftor n).
 
 Context `(sig: signature sig_sorts).
 
-
-
 Set Transparent Obligations.
 
-Equations lookup_tc_var ctx tys (tv: ty_valu ctx tys) (tc_var: ty_ctx_var ctx) : Type := {
+Equations lookup_tc_var {A} ctx (tys: snoc_list A) (tv: ty_valu ctx tys) (tc_var: ty_ctx_var ctx) : A := {
   lookup_tc_var _ _ (TVSnoc _ T _ _) (TCVHere _) := T; 
   lookup_tc_var _ _ (TVSnoc _ _ _ tv') (TCVThere _ tc_var') := lookup_tc_var _ _ tv' tc_var'; 
 }.
 
-Equations interp_te_var ctx tys (tv: ty_valu ctx tys) n (te_var: ty_expr_var sig_sorts ctx n) : arity_ftor n := {
+Equations interp_te_var ctx (tys: snoc_list Type) (tv: ty_valu ctx tys) n (te_var: ty_expr_var sig_sorts ctx n) : arity_ftor n := {
   interp_te_var _ _ tv _ (TEVAnon _ v) := 
     lookup_tc_var _ _ tv v;
   interp_te_var ctx _ _ n (TEVNamed _ _ f) := 
     interp_sorts _ f;
 }.
 
-Equations interp_te ctx tys (tv: ty_valu ctx tys) n (te: ty_expr sig_sorts ctx n) : arity_ftor n := {
+Equations interp_te ctx (tys: snoc_list Type) (tv: ty_valu ctx tys) n (te: ty_expr sig_sorts ctx n) : arity_ftor n := {
   interp_te _ _ tv n (TEVar _ v) := 
     interp_te_var _ _ tv n v;
   interp_te ctx tys tv _ (TEApp _ l r) := 
     let T := interp_te ctx tys tv _ r in 
       (interp_te ctx tys tv _ l) T;
 }.
+
+Equations apply_outer_params_tv
+  t_ctx_inner t_ctx_outer t_args (tys_outer: snoc_list Type)
+  (ty_args: ty_params sig_sorts t_ctx_outer t_ctx_inner t_args)
+  (tv_outer : ty_valu t_ctx_outer tys_outer) 
+  : ty_valu t_ctx_inner (sl_map (interp_te _ _ tv_outer 0) t_args) 
+    by struct ty_args := {
+  apply_outer_params_tv _ _ _ _ TVEmp _ := TVEmp;
+  apply_outer_params_tv _ _ _ _ (TVSnoc _ e _ tp') _ := TVSnoc _ _ _ (apply_outer_params_tv _ _ _ _ tp' _);
+}.
+
+Local Obligation Tactic := intros.
+Equations lookup_tvar_apply_eq {ctx t_ctx tys t_args tv} tp tvar :
+  interp_te t_ctx tys tv 0 (lookup_tp_var sig_sorts t_ctx ctx t_args tp tvar) =
+  lookup_tc_var ctx (sl_map (interp_te t_ctx tys tv 0) t_args) (apply_outer_params_tv ctx t_ctx t_args tys tp tv) tvar
+  by struct tvar := {
+  lookup_tvar_apply_eq (TVSnoc _ _ _ _) (TCVHere _) := eq_refl;
+  lookup_tvar_apply_eq (TVSnoc _ _ _ _) (TCVThere _ _) := _;
+}.
+Next Obligation.
+  autorewrite with lookup_tp_var.
+  autorewrite with apply_outer_params_tv.
+  simpl.
+  autorewrite with lookup_tc_var.
+  eapply lookup_tvar_apply_eq.
+Defined.
+
+Local Obligation Tactic := (unfold RelationClasses.complement, Equivalence.equiv; Tactics.program_simpl).
+
+Lemma apply_outer_eq:
+  forall n t_ctx t_ctx' tys t_args tp tv e, 
+    interp_te t_ctx tys tv n (apply_ty_args sig_sorts t_ctx' t_ctx t_args n tp e) 
+    = 
+    interp_te t_ctx' (sl_map (interp_te t_ctx tys tv 0) t_args) (apply_outer_params_tv t_ctx' t_ctx t_args tys tp tv) n e.
+Proof.
+induction e.
+  - simpl.
+    destruct t; autorewrite with apply_ty_args.
+    + autorewrite with interp_te.
+      autorewrite with interp_te_var.
+      eapply lookup_tvar_apply_eq.
+    + autorewrite with interp_te.
+      autorewrite with interp_te_var.
+      trivial.
+  - autorewrite with apply_ty_args.
+    unfold apply_ty_args_obligations_obligation_1, apply_ty_args_obligations_obligation_2, apply_ty_args_obligations_obligation_3, apply_ty_args_obligations_obligation_4.
+    autorewrite with interp_te.
+    simpl.
+    erewrite IHe2.
+    erewrite IHe1.
+    trivial.
+Defined.
+
 
 Record interp_sig (sig: signature sig_sorts) := {
   interp_funs: 
@@ -279,42 +263,69 @@ Context (model: interp_sig sig).
 
 Inductive valu ty_ctx tys (tv: ty_valu ty_ctx tys) : ctx sig_sorts ty_ctx -> Type := 
 | VEmp : 
-  valu ty_ctx tys tv (SLNil _)
+  valu ty_ctx tys tv SLNil
 | VSnoc : 
   forall sl e, 
     valu ty_ctx tys tv sl -> 
     interp_te ty_ctx tys tv 0 e ->
-    valu ty_ctx tys tv (Snoc _ sl e).
+    valu ty_ctx tys tv (Snoc sl e).
 
 Equations interp_var t_ctx tys tv e_ctx e (env: valu t_ctx tys tv e_ctx) (v: var sig_sorts _ e_ctx e) : interp_te t_ctx tys tv 0 e := {
   interp_var _ _ _ _ _ (VSnoc _ _ _ v) (VHere _ _ _ ) := v;
   interp_var _ _ _ _ _ (VSnoc _ _ env _) (VThere _ _ _ _ vi) := interp_var _ _ _ _ _ env vi;
 }.
 
-(* TODO: fix up interp_funs to handle type arguments. Need to consider how to adjust hargs, which is in the outer context, 
-    to the context of the inner function, which expects its own hargs.
-*)
+Set Transparent Obligations.
+(* Obligation Tactic := intros. *)
 Equations 
-  interp_tm t_ctx tys tv e_ctx e (env: valu t_ctx tys tv e_ctx) (t: tm sig_sorts sig t_ctx e_ctx e) : interp_te t_ctx tys tv 0 e by struct t := {
+  interp_tm 
+    t_ctx tys tv e_ctx e 
+    (env: valu t_ctx tys tv e_ctx) 
+    (t: tm sig_sorts sig t_ctx e_ctx e) 
+  : interp_te t_ctx tys tv 0 e 
+    by struct t 
+  := {
   interp_tm _ _ _ _ _ env (TVar _ _ v) := 
     interp_var _ _ _ _ _ env v;
-  interp_tm _ _ _ _ _ env (TFun _ _ _ _ _ f _ hargs) := 
-    model.(interp_funs sig) _ _ _ _ f _ (interp_tms _ _ _ _ env _ hargs);
+  interp_tm _ tys tv _ _ env (TFun _ t_args _ _ _ f tp hargs) :=
+    let inner := interp_tms _ _ tv _ env _ hargs in
+    let swapped := HList.map_swap _ _ inner in 
+    let trans_args := HList.map _ swapped in 
+    let inner_v := 
+      model.(interp_funs sig) _ (sl_map (interp_te _ _ tv 0) t_args) _ _ f (apply_outer_params_tv _ _ _ _ tp tv) trans_args in 
+    eq_rect_r (fun (x: arity_ftor 0) => x) inner_v (apply_outer_eq _ _ _ _ _ _ _ _);
+      (* interp_te_outer_params_apply _ inner_v; *)
+      (* _; *)
 } where 
-  interp_tms t_ctx ctx tv e_ctx (env: valu t_ctx ctx tv e_ctx) tys (tms: HList.t (tm sig_sorts sig t_ctx e_ctx) tys) : HList.t (interp_te t_ctx ctx tv 0) tys by struct tms := {
-  interp_tms _ _ _ _ _ _ hnil := 
-    hnil;
-  interp_tms _ _ _ _ _ _ (t ::: ts) := 
-    interp_tm _ _ _ _ _ _ t ::: interp_tms _ _ _ _ _ _ ts;
+  interp_tms 
+    t_ctx ctx tv e_ctx 
+    (env: valu t_ctx ctx tv e_ctx) tys 
+    (tms: HList.t 
+      (fun (te : ty_expr sig_sorts t_ctx 0) => 
+        tm sig_sorts sig t_ctx e_ctx te) 
+      tys
+    ) 
+  : HList.t (interp_te t_ctx ctx tv 0) tys by struct tms := {
+interp_tms _ _ _ _ _ _ hnil := 
+  hnil;
+interp_tms _ _ _ _ env _ (t ::: ts) := 
+  interp_tm _ _ _ _ _ _ t ::: interp_tms _ _ _ _ _ _ ts;
 }.
+Next Obligation.
+erewrite apply_outer_eq in X.
+apply X.
+Defined.
 
 Equations interp_fm t_ctx tys tv e_ctx (env: valu t_ctx tys tv e_ctx) (f: fm sig_sorts sig t_ctx e_ctx) : Prop := {
   interp_fm _ _ _ _ _ (FTrue _) := True;
   interp_fm _ _ _ _ _ (FFalse _) := False;
   interp_fm _ _ _ _ _ (FEq _ _ l r) := 
     (interp_tm _ _ _ _ _ _ l) = (interp_tm _ _ _ _ _ _ r);
-  interp_fm _ _ _ _ _ (FRel _ _ _ _ _ f hargs) := 
-    model.(interp_rels sig) _ _ _ f _ (interp_tms _ _ _ _ _ _ hargs);
+  interp_fm _ _ tv _ env (FRel _ t_args _ _ f tp hargs) :=
+    let inner := interp_tms _ _ tv _ env _ hargs in
+    let swapped := HList.map_swap _ _ inner in 
+    let trans_args := HList.map _ swapped in 
+      model.(interp_rels sig) _ (sl_map (interp_te _ _ tv 0) t_args) _ f (apply_outer_params_tv _ _ _ _ tp tv) trans_args;
   interp_fm _ _ _ _ _ (FAnd _ l r) := 
     interp_fm _ _ _ _ _ l /\ interp_fm _ _ _ _ _ r ;
   interp_fm _ _ _ _ _ (FOr _ l r) := 
@@ -332,8 +343,12 @@ Equations interp_fm t_ctx tys tv e_ctx (env: valu t_ctx tys tv e_ctx) (f: fm sig
     exists (x: interp_te t_ctx tys tv 0 e), 
       interp_fm _ _ _ _ (VSnoc _ _ _ _ _ env x) f ;
 }.
+Next Obligation.
+erewrite apply_outer_eq in X.
+apply X.
+Defined.
 
-Equations interp_pfm t_ctx tys (tv: ty_valu t_ctx tys) (pf: poly_fm sig_sorts sig t_ctx) : Prop := {
+Equations interp_pfm t_ctx (tys: snoc_list Type) (tv: ty_valu t_ctx tys) (pf: poly_fm sig_sorts sig t_ctx) : Prop := {
   interp_pfm t_ctx tys tv (PFm _ f) := 
     interp_fm t_ctx tys tv _ (VEmp _ _ _) f;
   interp_pfm t_ctx tys tv (PForall _ pf) := 
@@ -341,13 +356,26 @@ Equations interp_pfm t_ctx tys (tv: ty_valu t_ctx tys) (pf: poly_fm sig_sorts si
       interp_pfm _ _ (TVSnoc _ T _ _) pf;
 }.
 
+
 End PolySemantics.
+
 
 Arguments TEApp {_ _ _} _ _.
 Arguments TEVar {_ _ _} _.
 Arguments TEVAnon {_ _} _.
 Arguments TEVNamed {_ _ _} _.
 Arguments TCVHere {_}.
+
+Arguments PFm {_ _ _} _.
+Arguments PForall {_ _ _} _.
+Arguments FTrue {_ _ _ _}.
+Arguments FForall {_ _ _ _} _ _.
+Arguments FEq {_ _ _ _ _} _ _.
+Arguments TVar {_ _ _ _ _} _.
+Arguments VHere {_ _ _ _}.
+Arguments VThere {_ _ _ _ _} _.
+Arguments TFun {_ _ _ _ _ _ _ _} _ _ _.
+
 
 Section PolyDemo.
 
@@ -359,9 +387,11 @@ Inductive demo_sorts : nat -> Type :=
 | sort_list : demo_sorts 1
 | sort_nat : demo_sorts 0.
 
+Notation loc_A := (TEVar (TEVAnon TCVHere)).
+
 Notation list_A := (TEApp
   (TEVar (TEVNamed sort_list)) 
-  (TEVar (TEVAnon TCVHere))
+  loc_A
 ).
 
 Notation nat_ty := (TEVar (TEVNamed sort_nat)).
@@ -370,7 +400,8 @@ Inductive demo_funs :
   forall ctx, list (ty_expr demo_sorts ctx 0) -> ty_expr demo_sorts ctx 0 -> Type := 
 | demo_app : demo_funs 1 [list_A; list_A] list_A (* forall A, list A -> list A -> list A*)
 | demo_len : demo_funs 1 [list_A] nat_ty (* forall A, list A -> nat *)
-| demo_add : demo_funs 1 [nat_ty; nat_ty] nat_ty (* nat -> nat -> nat *)
+| demo_add : demo_funs 0 [nat_ty; nat_ty] nat_ty (* nat -> nat -> nat *)
+| demo_zero : demo_funs 0 [] nat_ty
 .
 
 Inductive demo_rels : 
@@ -393,6 +424,7 @@ Equations
   interp_demo_funs _ _ _ _ demo_app _ (l ::: r ::: _) := List.app l r; 
   interp_demo_funs _ _ _ _ demo_len _ (x ::: _) := List.length x; 
   interp_demo_funs _ _ _ _ demo_add _ (l ::: r ::: _) := l + r; 
+  interp_demo_funs _ _ _ _ demo_zero _ _ := 0; 
 }.
 
 Definition interp_demo_rels t_ctx ctx args (fn: demo_rels t_ctx args) tv (hargs: HList.t (interp_te demo_sorts interp_demo_sorts t_ctx ctx tv 0) args) : Prop := 
@@ -403,39 +435,64 @@ Program Definition demo_model : interp_sig demo_sorts interp_demo_sorts demo_sig
   interp_rels := interp_demo_rels;
 |}.
 
-Arguments PFm {_ _ _} _.
-Arguments PForall {_ _ _} _.
-Arguments FTrue {_ _ _ _}.
-Arguments FForall {_ _ _ _} _ _.
-Arguments FEq {_ _ _ _ _} _ _.
-Arguments TVar {_ _ _ _ _} _.
-Arguments VHere {_ _ _ _}.
-Arguments VThere {_ _ _ _ _} _.
-Arguments TFun {_ _ _ _ _ _} _ _.
+
+
 
 Notation t_xs := (TVar (VThere VHere)).
 Notation t_ys := (TVar VHere).
 
-Notation t_app args := (TFun (sig := demo_sig) demo_app args).
-Notation t_len args := (TFun (sig := demo_sig) demo_len args).
-Notation t_add args := (TFun (sig := demo_sig) demo_add args).
+Notation t_app ty_args args := (TFun (sig := demo_sig) demo_app ty_args args).
+Notation t_len ty_args args := (TFun (sig := demo_sig) demo_len ty_args args).
+Notation t_add args := (TFun (sig := demo_sig) demo_add TVEmp args).
+Notation t_zero := (TFun (sig := demo_sig) demo_zero TVEmp hnil).
 
-(* a polyfm version of app_len, i.e. 
-  forall A (xs ys: list A), 
-    length (xs ++ ys) = length xs + length ys *)
-Example app_len_pf: 
-  interp_pfm demo_sorts interp_demo_sorts demo_sig demo_model 0 (SLNil _) TVEmp
-  ( PForall (PFm (
+Program Definition app_len_pf_syntax: 
+  poly_fm demo_sorts demo_sig 0 :=  PForall (PFm (
     FForall list_A (FForall list_A (
       FEq 
-        (t_len (t_app (t_xs ::: t_ys ::: hnil) ::: hnil))
-        (t_add (t_len (t_xs ::: hnil) ::: (t_len (t_ys ::: hnil)) ::: hnil))
-    )))
+        (t_len _ ((t_app _ (t_xs ::: t_ys ::: hnil)) ::: hnil))
+        (t_add ((t_len (TVSnoc _ loc_A _ TVEmp) (t_xs ::: hnil)) ::: (t_len _ (t_ys ::: hnil)) ::: hnil))
+    ))
   )).
+
+Example app_len_pf: 
+  interp_pfm demo_sorts interp_demo_sorts demo_sig demo_model 0 SLNil TVEmp app_len_pf_syntax.
 Proof.
+  (* this short proof works as well: *)
+  (* 
   vm_compute.
   intros.
+  eapply List.app_length. 
+  *)
+  unfold app_len_pf_syntax.
+  autorewrite with interp_pfm.
+  unfold interp_pfm_obligations_obligation_1, interp_pfm_obligations_obligation_2.
+  intros.
+  autorewrite with interp_pfm.
+  autorewrite with interp_fm.
+  intros.
+  vm_compute in x.
+  autorewrite with interp_fm.
+  intros.
+  vm_compute in x0.
+  set (t := apply_ty_args _ _ _ _ _ _ _).
+  vm_compute in t.
+  subst t.
+  autorewrite with interp_fm.
+  unfold interp_fm_obligations_obligation_1, interp_fm_obligations_obligation_2, interp_fm_obligations_obligation_3, interp_fm_obligations_obligation_4.
+  set (t := apply_ty_args _ _ _ _ _ _ _);
+  vm_compute in t;
+  subst t.
+
+  set (l := interp_tm _ _ _ _ _ _ _ _ _ _ _).
+  set (r := interp_tm _ _ _ _ _ _ _ _ _ _ _).
+  vm_compute in l.
+  vm_compute in r.
   eapply List.app_length.
 Qed.
 
+(* Print Assumptions app_len_pf.  *)
+
 End PolyDemo.
+
+
